Update to LetNonRec.SSP

src/Language/PlutusIR/Transform/LetNonRec/SSP.v
@@ -17,51 +17,46 @@ Definition P_has_type Delta Gamma t1 T :=
 Definition P_constructor_well_formed Delta c T := Delta |-ok_c c : T.
 
 Definition P_bindings_well_formed_nonrec Delta Gamma bs1 :=
-    forall bs2, (
+  (
+    forall bs2,
       Delta ,, Gamma |-oks_nr bs1 ->
       Congruence.Cong_Bindings CNR_Term bs1 bs2 ->
-      Delta ,, Gamma |-oks_nr bs2
-    ) /\ (
-      Congruence.Cong_Bindings CNR_Term bs1 bs2 ->
-      map binds_Delta bs1 = map binds_Delta bs2 /\
-      map binds_Gamma bs1 = map binds_Gamma bs2
-    ) /\ (
-      forall f_bs2 t T bs1Gn,
-        Delta ,, Gamma |-oks_nr bs1 -> 
-        CNR_Bindings bs1 f_bs2 ->
-        map_normalise (flatten (map binds_Gamma bs1)) bs1Gn ->
-        (mupdate Delta (flatten (map binds_Delta bs1))) ,, (mupdate Gamma bs1Gn) |-+ t : T ->
-        Delta ,, Gamma |-+ (fold_right apply t f_bs2) : T
-    ).
-
-Definition P_bindings_well_formed_rec Delta Gamma bs1 :=
-  forall bs2, (
-    Delta ,, Gamma |-oks_r bs1 ->
-    Congruence.Cong_Bindings CNR_Term bs1 bs2 ->
-    Delta ,, Gamma |-oks_r bs2
+      Delta ,, Gamma |-oks_nr bs2 /\
+      map binds_Delta bs2 = map binds_Delta bs1 /\
+      map binds_Gamma bs2 = map binds_Gamma bs1
   ) /\ (
-    Congruence.Cong_Bindings CNR_Term bs1 bs2 ->
-    map binds_Delta bs1 = map binds_Delta bs2 /\
-    map binds_Gamma bs1 = map binds_Gamma bs2
+    forall f_bs2 t T bs1Gn,
+      Delta ,, Gamma |-oks_nr bs1 -> 
+      CNR_Bindings bs1 f_bs2 ->
+      map_normalise (flatten (map binds_Gamma bs1)) bs1Gn ->
+      (mupdate Delta (flatten (map binds_Delta bs1))) ,, (mupdate Gamma bs1Gn) |-+ t : T ->
+      Delta ,, Gamma |-+ (fold_right apply t f_bs2) : T
   ).
 
+Definition P_bindings_well_formed_rec Delta Gamma bs1 :=
+  forall bs2,
+    Delta ,, Gamma |-oks_r bs1 ->
+    Congruence.Cong_Bindings CNR_Term bs1 bs2 ->
+    Delta ,, Gamma |-oks_r bs2 /\
+    map binds_Delta bs2 = map binds_Delta bs1 /\
+    map binds_Gamma bs2 = map binds_Gamma bs1.
+
 Definition P_binding_well_formed Delta Gamma b1 := 
-  forall b2, (
+  (
+    forall b2,
       Delta ,, Gamma |-ok_b b1 ->
       Congruence.Cong_Binding CNR_Term b1 b2 ->
-      Delta ,, Gamma |-ok_b b2
-    ) /\ (
-      Congruence.Cong_Binding CNR_Term b1 b2 ->
-      binds_Delta b1 = binds_Delta b2 /\
-      binds_Gamma b1 = binds_Gamma b2
-    ) /\ (
-      forall f_b2 t T bs1Gn,
-        Delta ,, Gamma |-ok_b b1 ->
-        CNR_Binding b1 f_b2 ->
-        map_normalise (binds_Gamma b1) bs1Gn ->
-        mupdate Delta (binds_Delta b1) ,, mupdate Gamma bs1Gn |-+ t : T ->
-        Delta ,, Gamma |-+ (f_b2 t) : T  
-    ).
+      Delta ,, Gamma |-ok_b b2 /\
+      binds_Delta b2 = binds_Delta b1 /\
+      binds_Gamma b2 = binds_Gamma b1
+  ) /\ (
+    forall f_b2 t T bs1Gn,
+      Delta ,, Gamma |-ok_b b1 ->
+      CNR_Binding b1 f_b2 ->
+      map_normalise (binds_Gamma b1) bs1Gn ->
+      mupdate Delta (binds_Delta b1) ,, mupdate Gamma bs1Gn |-+ t : T ->
+      Delta ,, Gamma |-+ (f_b2 t) : T  
+  ).
 
 #[export] Hint Unfold
   P_has_type
@@ -85,195 +80,112 @@ Proof with (eauto with typing).
   all: try solve [eauto with typing].
   all: try solve [inversion X; subst; inversion X0; subst; eauto with typing].
   all: try solve [inversion X0; subst; inversion X1; subst; eauto with typing].
+  
   - (* T_Let *) 
     inversion X; subst.
     + eapply H3...
     + inversion X0; subst...
+      unfold P_bindings_well_formed_nonrec in H3.
+      destruct H3 as [[IHH [Heq Heq']] _]...
       eapply T_Let...
-      * unfold P_bindings_well_formed_nonrec in H3.
-        edestruct H3 as [_ [Heq _]].
-        apply Heq in X1.
-        destruct X1.
-        rewrite <- H1.
-        eassumption.
-      * apply H3...
-      * unfold P_bindings_well_formed_nonrec in H3. edestruct H3 as [_ [Heq _]]. apply Heq in X1. 
-        destruct X1. rewrite <- H. apply H5. assumption. 
+      * rewrite Heq'...
+      * rewrite Heq...
   - (* T_LetRec *)
     inversion X. subst.
     inversion X0. subst.
+    unfold P_bindings_well_formed_rec in H3.
+    edestruct H3 as [IHH [Heq Heq']]...
     eapply T_LetRec...
-    + unfold P_bindings_well_formed_rec in H3.
-      edestruct H3 as [IHH Heq].
-      apply Heq in X1 as Hsu.
-      destruct Hsu.
-      rewrite <- H1.
-      eassumption.
-    + unfold P_bindings_well_formed_rec in H3.
-      edestruct H3 as [IHH Heq].
-      apply Heq in X1 as Hsu.
-      destruct Hsu.
-      rewrite <- H.
-      apply IHH. auto. auto.
-    + unfold P_bindings_well_formed_rec in H3.
-      edestruct H3 as [IHH Heq].
-      apply Heq in X1 as Hsu.
-      destruct Hsu.
-      rewrite <- H.
-      apply H5.
-      assumption.
+    + rewrite Heq'...
+    + rewrite Heq...
+    + rewrite Heq...
     
   - (* W_NilB_NonRec *)
-    split.
-    + intros.
-      inversion X. subst.
-      assumption.
-    + split.
-      * intros.
-        inversion X. subst.
-        auto.
-      * intros.
-        inversion X. subst.
-        simpl in H0.
-        inversion H0. subst.
-        assumption.
+    split. all: intros.
+    + inversion X... 
+    + inversion X.
+      inversion H0.
+      subst...
   - (* W_ConsB_NonRec *)
-    split.
-    + intros.
-      inversion X. subst.
-      eapply W_ConsB_NonRec.
-      * apply H0. assumption. assumption.
-      * unfold P_binding_well_formed in H0.
-        edestruct H0 as [_ [Heq _]].
-        apply Heq in X0.
-        destruct X0.
-        rewrite <- H6.
-        eassumption.
-      * unfold P_binding_well_formed in H0.
-        edestruct H0 as [_ [Heq _]].
-        apply Heq in X0.
-        destruct X0.
-        rewrite <- H5.
-        apply H3. assumption. assumption.
-    + split.
-      * intros.
-        inversion X. subst.
-        simpl.
-        split.
-        -- f_equal.
-           ++ apply H0. assumption.
-           ++ apply H3. assumption.
-        -- f_equal.
-           ++ apply H0. assumption.
-           ++ apply H3. assumption.
-      * intros.
-        inversion X. subst.
-        inversion X0. subst.
-        edestruct H3 as [_ [_ J]].
-        
-        simpl.
-        edestruct H0 as [_ [_ J2]].
-        eapply J2.
-        -- assumption.
-        -- assumption.
-        -- eassumption.
-        -- unfold flatten in H5.
-            simpl in H5.
-            rewrite concat_app in H5.
-            simpl in H5.
-            apply map_normalise__app in H5 as H20. 
-            destruct H20 as [l1n [l2n [Hmn1 [Hmn2 Heq]]]].
-            subst. 
-
-          eapply J.
-           ++ assumption.
-           ++ assumption.
-           ++ eauto.
-           ++ simpl.
-              simpl in H6.
-              unfold flatten in H6.
-              simpl in H6.  
-              rewrite concat_app in H6.
-              simpl in H6.
-              rewrite app_nil_r in H6.
-              rewrite mupdate_app in H6.
-              simpl in H6.
-              simpl in H1.
-              eapply map_normalise__deterministic in H1; eauto.
-              subst.
-              apply H6.
-  - (* W_NilB_Rec *)
-    split.
-    + intros.
-      inversion X. subst.
-      assumption.
-    + intros.
-      inversion X. subst.
-      auto.
-  - (* W_ConsB_Rec*)
-    split.
-    + intros.
-      inversion X. subst.
-      apply W_ConsB_Rec.
-      * apply H0. assumption. assumption.
-      * apply H2. assumption. assumption.
-    + intros.
-      inversion X. subst.
+    split. all: intros.
+    + inversion X. subst.
+      unfold P_binding_well_formed in H0.
+      destruct H0 as [[IH [Heq Heq']] _]...
+      split; try split.
+      * eapply W_ConsB_NonRec...
+        -- rewrite Heq'...
+        -- rewrite Heq... eapply H3...
+      * simpl. rewrite Heq...
+        f_equal. eapply H3...
+      * simpl. rewrite Heq'...
+        f_equal. eapply H3...
+    + inversion X. subst.
+      inversion X0. subst.
+      destruct H0 as [_ IH1]...
+      destruct H3 as [_ IH2]...
       simpl.
-      split.
-      -- f_equal.
-         ++ apply H0. assumption.
-         ++ apply H2. assumption.
-      -- f_equal.
-         ++ apply H0. assumption.
-         ++ apply H2. assumption.
+
+      simpl in H5.
+      unfold flatten in H5.
+      simpl in H5.
+      rewrite concat_app in H5.
+      simpl in H5.
+      apply map_normalise__app in H5 as H7.
+      destruct H7 as [l1n [l2n [Hn__l1n [H1__l2n Heql]]]].
+      simpl in H1__l2n.
+      inversion H1__l2n. subst.
+      inversion H9. subst.
+
+      simpl in H1.
+      inversion H1. subst.
+      inversion H11. subst.
+
+      eapply normalisation__deterministic in H10...
+      subst.
+
+      eapply IH1...
+      eapply IH2...
+
+      simpl in H6.
+      rewrite mupdate_app in H6.
+      unfold flatten in H6.
+      simpl in H6.
+      rewrite concat_app in H6.
+      simpl in H6.
+      rewrite app_nil_r in H6.
+
+      eapply H6.
+
+  - (* W_NilB_Rec *)
+    inversion X. subst.
+    eauto.
+  - (* W_ConsB_Rec*)
+    inversion X. subst.
+    unfold P_binding_well_formed in H0.
+    destruct H0 as [[IH [Heq Heq']] _]...
+    split; try split.
+    + eapply W_ConsB_Rec...
+      eapply H2...
+    + simpl. rewrite Heq...
+      f_equal. eapply H2...
+    + simpl. rewrite Heq'...
+      f_equal. eapply H2...
            
   - (* W_Term *)
-    split.
-    + intros. 
-      inversion X. subst.
-      eapply W_Term...
-    + split. 
-      * intros.
-        inversion X. subst.
-        auto.
-      * intros.
-        inversion X. subst.
-        eapply T_Apply...
-        apply T_LamAbs...
-        simpl in H4.
-        inversion H4. subst.
-        inversion H10. subst.
-        eapply normalisation__deterministic in H0; eauto.
-        subst.
-        inversion H3. subst.
-        simpl in H3.
-        inversion H3. subst.
-        inversion H10. subst.
-        eassumption.
+    split. all: intros.
+    + inversion X. subst...
+    + inversion X. subst...
+      simpl in H4.
+      inversion H4. subst.
+      inversion H10. subst.
+      eapply normalisation__deterministic in H0...
+      subst...
   - (* W_Type *)
-    split.
-    + intros. 
-      inversion X0. subst.
-      apply W_Type.
-      assumption.
-    + split.
-      * intros.
-        inversion X0. subst.
-        auto.
-      * intros.
-        inversion X0.
+    split. all: intros.
+    + inversion X0. subst...
+    + inversion X0.
   - (* W_Data *)
-    split.
-    + intros.
-      inversion X0. subst.
-      assumption.
-    + split.
-      * intros.
-        inversion X0. subst.
-        auto.
-      * intros.
-        inversion X0.
-
-  Unshelve. auto. apply (TermBind Strict (VarDecl v ty) t_bound).
+    split. all: intros.
+    + inversion X0. subst...
+    + inversion X0.
 Qed. 
